Manually proved the derivability of Peterson's algorithm

Example2.thy
@@ -38,53 +38,78 @@ definition Equal::"aexp \<Rightarrow> aexp \<Rightarrow> bexp" where "Equal a1 a
 lemma or_bval:"bval (Or b1 b2) s = (bval b1 s \<or> bval b2 s)" by (metis Or_def bval.simps(2) bval_And_if)
 lemma equal_bval:"bval (Equal a1 a2) s = (aval a1 s = aval a2 s)" by (smt Equal_def bval.simps(2) bval.simps(4) bval_And_if) 
 
-abbreviation pre10 :: "assn" where "pre10 \<equiv> \<lambda>s. s ''f0'' = 0"
-abbreviation pre11 :: "assn" where "pre11 \<equiv> \<lambda>s. s ''f0'' = 1"
-abbreviation pre12 :: "assn" where "pre12 \<equiv> \<lambda>s. s ''f0'' = 1 \<and> (s ''t'' = 1 \<or> s ''t'' = 0)"
-abbreviation pre13 :: "assn" where "pre13 \<equiv> \<lambda>s. s ''f0'' = 1 \<and> (s ''f1'' = 0 \<or> s ''t'' = 0)"
+abbreviation pre10 :: "assn" where "pre10 \<equiv> \<lambda>s. s ''f0'' = 0 \<and> s ''d0'' = 0 \<and> (s ''d1'' = 0 \<longrightarrow> s ''f1'' = 0)
+  \<and> (s ''d1'' = 1 \<longrightarrow> s ''f1'' = 1) \<and> (s ''d1'' = 2 \<longrightarrow> (s ''f1'' = 1 \<and> s ''t'' = 0)) \<and> (s ''d1'' = 3 \<longrightarrow> (s ''f1'' = 1 \<and> s ''t'' = 0))
+  \<and> (s ''d1'' = 4 \<longrightarrow> s ''f1'' = 0)"
+abbreviation pre11 :: "assn" where "pre11 \<equiv> \<lambda>s. s ''f0'' = 1 \<and> s ''d0'' = 1 \<and> (s ''d1'' = 0 \<longrightarrow> s ''f1'' = 0)
+  \<and> (s ''d1'' = 1 \<longrightarrow> s ''f1'' = 1) \<and> (s ''d1'' = 2 \<longrightarrow> (s ''f1'' = 1 \<and> s ''t'' = 0)) \<and> (s ''d1'' = 3 \<longrightarrow> (s ''f1'' = 1 \<and> s ''t'' = 0))
+  \<and> (s ''d1'' = 4 \<longrightarrow> s ''f1'' = 0)"
+abbreviation pre12 :: "assn" where "pre12 \<equiv> \<lambda>s. s ''f0'' = 1 \<and> s ''d0'' = 2 \<and> (s ''d1'' = 0 \<longrightarrow> s ''f1'' = 0)
+  \<and> (s ''d1'' = 1 \<longrightarrow> s ''f1'' = 1) \<and> (s ''d1'' = 2 \<longrightarrow> (s ''f1'' = 1 \<and> (s ''t'' = 0 \<or> s ''t'' = 1))) 
+  \<and> (s ''d1'' = 3 \<longrightarrow> (s ''f1'' = 1 \<and> s ''t'' = 1)) \<and> (s ''d1'' = 4 \<longrightarrow> s ''f1'' = 0)"
+abbreviation pre13 :: "assn" where "pre13 \<equiv> \<lambda>s. s ''f0'' = 1 \<and> s ''d0'' = 2 \<and> (s ''d1'' = 0 \<longrightarrow> s ''f1'' = 0)
+  \<and> (s ''d1'' = 1 \<longrightarrow> s ''f1'' = 1) \<and> (s ''d1'' = 2 \<longrightarrow> (s ''f1'' = 1 \<and> s ''t'' = 0)) 
+  \<and> (s ''d1'' = 3 \<longrightarrow> False) \<and> (s ''d1'' = 4 \<longrightarrow> s ''f1'' = 0)"
+abbreviation pre14 :: "assn" where "pre14 \<equiv> \<lambda>s. s ''f0'' = 1 \<and> s ''d0'' = 3 \<and> (s ''d1'' = 0 \<longrightarrow> s ''f1'' = 0)
+  \<and> (s ''d1'' = 1 \<longrightarrow> s ''f1'' = 1) \<and> (s ''d1'' = 2 \<longrightarrow> (s ''f1'' = 1 \<and> s ''t'' = 0)) 
+  \<and> (s ''d1'' = 3 \<longrightarrow> False) \<and> (s ''d1'' = 4 \<longrightarrow> s ''f1'' = 0)"
 
-abbreviation assign11  :: "state \<Rightarrow> state" where "assign11 \<equiv> \<lambda>s. s(''f0'' := 1)"
-abbreviation assign12  :: "state \<Rightarrow> state" where "assign12 \<equiv> \<lambda>s. s(''t'' := 1)"
-abbreviation assign13  :: "state \<Rightarrow> state" where "assign13 \<equiv> \<lambda>s. s(''f0'' := 0)"
+abbreviation assign11  :: "state \<Rightarrow> state" where "assign11 \<equiv> \<lambda>s. s(''f0'' := 1, ''d0'' := s ''d0'' + 1)"
+abbreviation assign12  :: "state \<Rightarrow> state" where "assign12 \<equiv> \<lambda>s. s(''t'' := 1, ''d0'' := s ''d0'' + 1)"
+abbreviation assign13  :: "state \<Rightarrow> state" where "assign13 \<equiv> \<lambda>s. s(''d0'' := s ''d0'' + 1)"
+abbreviation assign14  :: "state \<Rightarrow> state" where "assign14 \<equiv> \<lambda>s. s(''f0'' := 0, ''d0'' := s ''d0'' + 1)"
+
+abbreviation post1 :: "assn" where "post1 \<equiv> \<lambda>s. s ''f0'' = 0 \<and> s ''d0'' = 4"
 
 abbreviation p1::"acom" where "p1 \<equiv> (((((ABasic (pre10) assign11);; ABasic (pre11) assign12);;
-({pre12} WAIT (Or (Equal (V ''f1'') (N 0)) (Equal (V ''t'') (N 0))) END));; (ABasic (pre13) id));; (ABasic (pre13) assign13))"
+({pre12} WAIT (Or (Equal (V ''f1'') (N 0)) (Equal (V ''t'') (N 0))) END));; (ABasic (pre13) assign13));; (ABasic (pre14) assign14))"
 
-lemma atomic_p1:"(atomics p1) = {(pre10, Basic assign11),(pre11, Basic assign12),(pre13, Basic id),(pre13, Basic assign13)}"
+lemma atomic_p1:"(atomics p1) = {(pre10, Basic assign11),(pre11, Basic assign12),(pre13, Basic assign13),(pre14, Basic assign14)}"
 by (simp add: insert_commute)
 
-lemma assertion_p1:"(assertions p1) = {pre10, pre11, pre12, pre13, pre13}" by auto
+lemma assertion_p1:"(assertions p1) = {pre10, pre11, pre12, pre13, pre14}" by auto
 
-abbreviation pre20 :: "assn" where "pre20 \<equiv> \<lambda>s. s ''f1'' = 0"
-abbreviation pre21 :: "assn" where "pre21 \<equiv> \<lambda>s. s ''f1'' = 1"
-abbreviation pre22 :: "assn" where "pre22 \<equiv> \<lambda>s. s ''t'' = 0 \<and> s ''f1'' = 1"
-abbreviation pre23 :: "assn" where "pre23 \<equiv> \<lambda>s. s ''f1'' = 1 \<and> (s ''f0'' = 0 \<or> s ''t'' = 1)"
+abbreviation pre20 :: "assn" where "pre20 \<equiv> \<lambda>s. s ''f1'' = 0 \<and> s ''d1'' = 0 \<and> (s ''d0'' = 0 \<longrightarrow> s ''f0'' = 0)
+  \<and> (s ''d0'' = 1 \<longrightarrow> s ''f0'' = 1) \<and> (s ''d0'' = 2 \<longrightarrow> (s ''f0'' = 1 \<and> s ''t'' = 1)) \<and> (s ''d0'' = 3 \<longrightarrow> (s ''f0'' = 1 \<and> s ''t'' = 1))
+  \<and> (s ''d0'' = 4 \<longrightarrow> s ''f0'' = 0)"
+abbreviation pre21 :: "assn" where "pre21 \<equiv> \<lambda>s. s ''f1'' = 1 \<and> s ''d1'' = 1 \<and> (s ''d0'' = 0 \<longrightarrow> s ''f0'' = 0)
+  \<and> (s ''d0'' = 1 \<longrightarrow> s ''f0'' = 1) \<and> (s ''d0'' = 2 \<longrightarrow> (s ''f0'' = 1 \<and> s ''t'' = 1)) \<and> (s ''d0'' = 3 \<longrightarrow> (s ''f0'' = 1 \<and> s ''t'' = 1))
+  \<and> (s ''d0'' = 4 \<longrightarrow> s ''f0'' = 0)"
+abbreviation pre22 :: "assn" where "pre22 \<equiv> \<lambda>s. s ''f1'' = 1 \<and> s ''d1'' = 2 \<and> (s ''d0'' = 0 \<longrightarrow> s ''f0'' = 0)
+  \<and> (s ''d0'' = 1 \<longrightarrow> s ''f0'' = 1) \<and> (s ''d0'' = 2 \<longrightarrow> (s ''f0'' = 1 \<and> (s ''t'' = 0 \<or> s ''t'' = 1))) 
+  \<and> (s ''d0'' = 3 \<longrightarrow> (s ''f0'' = 1 \<and> s ''t'' = 0)) \<and> (s ''d0'' = 4 \<longrightarrow> s ''f0'' = 0)"
+abbreviation pre23 :: "assn" where "pre23 \<equiv> \<lambda>s. s ''f1'' = 1 \<and> s ''d1'' = 2 \<and> (s ''d0'' = 0 \<longrightarrow> s ''f0'' = 0)
+  \<and> (s ''d0'' = 1 \<longrightarrow> s ''f0'' = 1) \<and> (s ''d0'' = 2 \<longrightarrow> (s ''f0'' = 1 \<and> s ''t'' = 1)) 
+  \<and> (s ''d0'' = 3 \<longrightarrow> False) \<and> (s ''d0'' = 4 \<longrightarrow> s ''f0'' = 0)"
+abbreviation pre24 :: "assn" where "pre24 \<equiv> \<lambda>s. s ''f1'' = 1 \<and> s ''d1'' = 3 \<and> (s ''d0'' = 0 \<longrightarrow> s ''f0'' = 0)
+  \<and> (s ''d0'' = 1 \<longrightarrow> s ''f0'' = 1) \<and> (s ''d0'' = 2 \<longrightarrow> (s ''f0'' = 1 \<and> s ''t'' = 1)) 
+  \<and> (s ''d0'' = 3 \<longrightarrow> False) \<and> (s ''d0'' = 4 \<longrightarrow> s ''f0'' = 0)"
 
-abbreviation assign21  :: "state \<Rightarrow> state" where "assign21 \<equiv> \<lambda>s. s(''f1'' := 1)"
-abbreviation assign22  :: "state \<Rightarrow> state" where "assign22 \<equiv> \<lambda>s. s(''t'' := 0)"
-abbreviation assign23  :: "state \<Rightarrow> state" where "assign23 \<equiv> \<lambda>s. s(''f1'' := 0)"
+abbreviation assign21  :: "state \<Rightarrow> state" where "assign21 \<equiv> \<lambda>s. s(''f1'' := 1, ''d1'' := s ''d1'' + 1)"
+abbreviation assign22  :: "state \<Rightarrow> state" where "assign22 \<equiv> \<lambda>s. s(''t'' := 0, ''d1'' := s ''d1'' + 1)"
+abbreviation assign23  :: "state \<Rightarrow> state" where "assign23 \<equiv> \<lambda>s. s(''d1'' := s ''d1'' + 1)"
+abbreviation assign24  :: "state \<Rightarrow> state" where "assign24 \<equiv> \<lambda>s. s(''f1'' := 0, ''d1'' := s ''d1'' + 1)"
 
-abbreviation post1 :: "assn" where "post1 \<equiv> \<lambda>s. s ''f0'' = 0"
-abbreviation post2 :: "assn" where "post2 \<equiv> \<lambda>s. s ''f1'' = 0"
+abbreviation post2 :: "assn" where "post2 \<equiv> \<lambda>s. s ''f1'' = 0 \<and> s ''d1'' = 4"
 
 abbreviation p2::"acom" where "p2 \<equiv> (((((ABasic (pre20) assign21);; ABasic (pre21) assign22);;
-({pre22} WAIT (Or (Equal (V ''f0'') (N 0)) (Equal (V ''t'') (N 1))) END));; (ABasic (pre23) id));; (ABasic (pre23) assign23))"
+({pre22} WAIT (Or (Equal (V ''f0'') (N 0)) (Equal (V ''t'') (N 1))) END));; (ABasic (pre23) assign23));; (ABasic (pre24) assign24))"
 
-lemma atomic_p2:"(atomics p2) = {(pre20, Basic assign21),(pre21, Basic assign22),(pre23, Basic id),(pre23, Basic assign23)}"
+lemma atomic_p2:"(atomics p2) = {(pre20, Basic assign21),(pre21, Basic assign22),(pre23, Basic assign23),(pre24, Basic assign24)}"
 by (simp add: insert_commute)
 
-lemma assertion_p2:"(assertions p2) = {pre20, pre21, pre22, pre23, pre23}" by auto
+lemma assertion_p2:"(assertions p2) = {pre20, pre21, pre22, pre23, pre24}" by auto
 
 lemma p1_hoare:"\<turnstile> p1 {post1}"
 proof -
   have "vc p1 post1" using equal_bval or_bval by auto
-  thus ?thesis by simp
+  thus ?thesis by (meson vc_sound)
 qed
 
 lemma p2_hoare:"\<turnstile> p2 {post2}"
 proof -
   have "vc p2 post2" using equal_bval or_bval by auto
-  thus ?thesis by simp
+  thus ?thesis by (meson vc_sound)
 qed
 
 lemma interf_21_post:"\<forall>(R, r) \<in> (atomics p2). \<Turnstile>\<^sub>t\<^sub>r {\<lambda>s. post1 s \<and> R s} r {post1}"
@@ -93,23 +118,57 @@ proof -
   hence 1:"\<Turnstile>\<^sub>t\<^sub>r {\<lambda>s. post1 s \<and> pre20 s} Basic assign21 {post1}" using hoare_sound_tr by blast
   have "\<turnstile>\<^sub>t\<^sub>r {\<lambda>s. post1 s \<and> pre21 s} Basic assign22 {post1}" by simp
   hence 2:"\<Turnstile>\<^sub>t\<^sub>r {\<lambda>s. post1 s \<and> pre21 s} Basic assign22 {post1}" using hoare_sound_tr by blast
-  have "\<turnstile>\<^sub>t\<^sub>r {\<lambda>s. post1 s \<and> pre23 s} Basic id {post1}" by simp
-  hence 3:"\<Turnstile>\<^sub>t\<^sub>r {\<lambda>s. post1 s \<and> pre23 s} Basic id {post1}" using hoare_sound_tr by blast
   have "\<turnstile>\<^sub>t\<^sub>r {\<lambda>s. post1 s \<and> pre23 s} Basic assign23 {post1}" by simp
-  hence 4:"\<Turnstile>\<^sub>t\<^sub>r {\<lambda>s. post1 s \<and> pre23 s} Basic assign23 {post1}" using hoare_sound_tr by blast
+  hence 3:"\<Turnstile>\<^sub>t\<^sub>r {\<lambda>s. post1 s \<and> pre23 s} Basic assign23 {post1}" using hoare_sound_tr by blast
+  have "\<turnstile>\<^sub>t\<^sub>r {\<lambda>s. post1 s \<and> pre24 s} Basic assign24 {post1}" by simp
+  hence 4:"\<Turnstile>\<^sub>t\<^sub>r {\<lambda>s. post1 s \<and> pre24 s} Basic assign24 {post1}" using hoare_sound_tr by blast
   show ?thesis using 1 2 3 4 atomic_p1 by simp
 qed
 
-(*lemma atomic_p2:"(atomics p2) = {(pre20, Basic assign21),(pre21, Basic assign22),(pre23, Basic id),(pre23, Basic assign23)}"
-by (simp add: insert_commute)*)
-(*lemma assertion_p1:"(assertions p1) = {pre0, pre11, pre12, pre13, pre13}" by auto*)
 lemma interf_21_pre:"\<forall>(R, r) \<in> (atomics p2).(\<forall>P \<in> (assertions p1).\<Turnstile>\<^sub>t\<^sub>r {\<lambda>s. P s \<and> R s} r {P})"
 proof-
   have "\<turnstile>\<^sub>t\<^sub>r {\<lambda>s. pre10 s \<and> pre20 s} Basic assign21 {pre10}" by simp
   hence 1:"\<Turnstile>\<^sub>t\<^sub>r {\<lambda>s. pre10 s \<and> pre20 s} Basic assign21 {pre10}" using hoare_sound_tr by blast
   have "\<turnstile>\<^sub>t\<^sub>r {\<lambda>s. pre11 s \<and> pre20 s} Basic assign21 {pre11}" by simp
   hence 2:"\<Turnstile>\<^sub>t\<^sub>r {\<lambda>s. pre11 s \<and> pre20 s} Basic assign21 {pre11}" using hoare_sound_tr by blast
-oops
+  have "\<turnstile>\<^sub>t\<^sub>r {\<lambda>s. pre12 s \<and> pre20 s} Basic assign21 {pre12}" by simp
+  hence 3:"\<Turnstile>\<^sub>t\<^sub>r {\<lambda>s. pre12 s \<and> pre20 s} Basic assign21 {pre12}" using hoare_sound_tr by blast
+  have "\<turnstile>\<^sub>t\<^sub>r {\<lambda>s. pre13 s \<and> pre20 s} Basic assign21 {pre13}" by simp
+  hence 4:"\<Turnstile>\<^sub>t\<^sub>r {\<lambda>s. pre13 s \<and> pre20 s} Basic assign21 {pre13}" using hoare_sound_tr by blast
+  have "\<turnstile>\<^sub>t\<^sub>r {\<lambda>s. pre14 s \<and> pre20 s} Basic assign21 {pre14}" by simp
+  hence 5:"\<Turnstile>\<^sub>t\<^sub>r {\<lambda>s. pre14 s \<and> pre20 s} Basic assign21 {pre14}" using hoare_sound_tr by blast
+  have "\<turnstile>\<^sub>t\<^sub>r {\<lambda>s. pre10 s \<and> pre21 s} Basic assign22 {pre10}" by simp
+  hence 6:"\<Turnstile>\<^sub>t\<^sub>r {\<lambda>s. pre10 s \<and> pre21 s} Basic assign22 {pre10}" using hoare_sound_tr by blast
+  have "\<turnstile>\<^sub>t\<^sub>r {\<lambda>s. pre11 s \<and> pre21 s} Basic assign22 {pre11}" by simp
+  hence 7:"\<Turnstile>\<^sub>t\<^sub>r {\<lambda>s. pre11 s \<and> pre21 s} Basic assign22 {pre11}" using hoare_sound_tr by blast
+  have "\<turnstile>\<^sub>t\<^sub>r {\<lambda>s. pre12 s \<and> pre21 s} Basic assign22 {pre12}" by simp
+  hence 8:"\<Turnstile>\<^sub>t\<^sub>r {\<lambda>s. pre12 s \<and> pre21 s} Basic assign22 {pre12}" using hoare_sound_tr by blast
+  have "\<turnstile>\<^sub>t\<^sub>r {\<lambda>s. pre13 s \<and> pre21 s} Basic assign22 {pre13}" by simp
+  hence 9:"\<Turnstile>\<^sub>t\<^sub>r {\<lambda>s. pre13 s \<and> pre21 s} Basic assign22 {pre13}" using hoare_sound_tr by blast
+  have "\<turnstile>\<^sub>t\<^sub>r {\<lambda>s. pre14 s \<and> pre21 s} Basic assign22 {pre14}" by simp
+  hence 10:"\<Turnstile>\<^sub>t\<^sub>r {\<lambda>s. pre14 s \<and> pre21 s} Basic assign22 {pre14}" using hoare_sound_tr by blast
+  have "\<turnstile>\<^sub>t\<^sub>r {\<lambda>s. pre10 s \<and> pre23 s} Basic assign23 {pre10}" by simp
+  hence 11:"\<Turnstile>\<^sub>t\<^sub>r {\<lambda>s. pre10 s \<and> pre23 s} Basic assign23 {pre10}" using hoare_sound_tr by blast
+  have "\<turnstile>\<^sub>t\<^sub>r {\<lambda>s. pre11 s \<and> pre23 s} Basic assign23 {pre11}" by simp
+  hence 12:"\<Turnstile>\<^sub>t\<^sub>r {\<lambda>s. pre11 s \<and> pre23 s} Basic assign23 {pre11}" using hoare_sound_tr by blast
+  have "\<turnstile>\<^sub>t\<^sub>r {\<lambda>s. pre12 s \<and> pre23 s} Basic assign23 {pre12}" by simp
+  hence 13:"\<Turnstile>\<^sub>t\<^sub>r {\<lambda>s. pre12 s \<and> pre23 s} Basic assign23 {pre12}" using hoare_sound_tr by blast
+  have "\<turnstile>\<^sub>t\<^sub>r {\<lambda>s. pre13 s \<and> pre23 s} Basic assign23 {pre13}" by simp
+  hence 14:"\<Turnstile>\<^sub>t\<^sub>r {\<lambda>s. pre13 s \<and> pre23 s} Basic assign23 {pre13}" using hoare_sound_tr by blast
+  have "\<turnstile>\<^sub>t\<^sub>r {\<lambda>s. pre14 s \<and> pre23 s} Basic assign23 {pre14}" by simp
+  hence 15:"\<Turnstile>\<^sub>t\<^sub>r {\<lambda>s. pre14 s \<and> pre23 s} Basic assign23 {pre14}" using hoare_sound_tr by blast
+  have "\<turnstile>\<^sub>t\<^sub>r {\<lambda>s. pre10 s \<and> pre24 s} Basic assign24 {pre10}" by simp
+  hence 16:"\<Turnstile>\<^sub>t\<^sub>r {\<lambda>s. pre10 s \<and> pre24 s} Basic assign24 {pre10}" using hoare_sound_tr by blast
+  have "\<turnstile>\<^sub>t\<^sub>r {\<lambda>s. pre11 s \<and> pre24 s} Basic assign24 {pre11}" by simp
+  hence 17:"\<Turnstile>\<^sub>t\<^sub>r {\<lambda>s. pre11 s \<and> pre24 s} Basic assign24 {pre11}" using hoare_sound_tr by blast
+  have "\<turnstile>\<^sub>t\<^sub>r {\<lambda>s. pre12 s \<and> pre24 s} Basic assign24 {pre12}" by simp
+  hence 18:"\<Turnstile>\<^sub>t\<^sub>r {\<lambda>s. pre12 s \<and> pre24 s} Basic assign24 {pre12}" using hoare_sound_tr by blast
+  have "\<turnstile>\<^sub>t\<^sub>r {\<lambda>s. pre13 s \<and> pre24 s} Basic assign24 {pre13}" by simp
+  hence 19:"\<Turnstile>\<^sub>t\<^sub>r {\<lambda>s. pre13 s \<and> pre24 s} Basic assign24 {pre13}" using hoare_sound_tr by blast
+  have "\<turnstile>\<^sub>t\<^sub>r {\<lambda>s. pre14 s \<and> pre24 s} Basic assign24 {pre14}" by simp
+  hence 20:"\<Turnstile>\<^sub>t\<^sub>r {\<lambda>s. pre14 s \<and> pre24 s} Basic assign24 {pre14}" using hoare_sound_tr by blast
+  show ?thesis using 1 2 3 4 5 6 7 8 9 10 11 12 13 14 15 16 17 18 19 20 by auto
+qed
   
 
 lemma interf_12_post:"\<forall>(R, r) \<in> (atomics p1). \<Turnstile>\<^sub>t\<^sub>r {\<lambda>s. post2 s \<and> R s} r {post2}"
@@ -118,18 +177,61 @@ proof -
   hence 1:"\<Turnstile>\<^sub>t\<^sub>r {\<lambda>s. post2 s \<and> pre10 s} Basic assign11 {post2}" using hoare_sound_tr by blast
   have "\<turnstile>\<^sub>t\<^sub>r {\<lambda>s. post2 s \<and> pre11 s} Basic assign12 {post2}" by simp
   hence 2:"\<Turnstile>\<^sub>t\<^sub>r {\<lambda>s. post2 s \<and> pre11 s} Basic assign12 {post2}" using hoare_sound_tr by blast
-  have "\<turnstile>\<^sub>t\<^sub>r {\<lambda>s. post2 s \<and> pre13 s} Basic id {post2}" by simp
-  hence 3:"\<Turnstile>\<^sub>t\<^sub>r {\<lambda>s. post2 s \<and> pre13 s} Basic id {post2}" using hoare_sound_tr by blast
   have "\<turnstile>\<^sub>t\<^sub>r {\<lambda>s. post2 s \<and> pre13 s} Basic assign13 {post2}" by simp
-  hence 4:"\<Turnstile>\<^sub>t\<^sub>r {\<lambda>s. post2 s \<and> pre13 s} Basic assign13 {post2}" using hoare_sound_tr by blast
+  hence 3:"\<Turnstile>\<^sub>t\<^sub>r {\<lambda>s. post2 s \<and> pre13 s} Basic assign13 {post2}" using hoare_sound_tr by blast
+  have "\<turnstile>\<^sub>t\<^sub>r {\<lambda>s. post2 s \<and> pre14 s} Basic assign14 {post2}" by simp
+  hence 4:"\<Turnstile>\<^sub>t\<^sub>r {\<lambda>s. post2 s \<and> pre14 s} Basic assign14 {post2}" using hoare_sound_tr by blast
   show ?thesis using 1 2 3 4 atomic_p2 by simp
 qed
 
-lemma interf_12_pre:"\<forall>(R, r) \<in> (atomics p1).(\<forall>P \<in> (assertions p2).\<Turnstile>\<^sub>t\<^sub>r {\<lambda>s. P s \<and> R s} r {P})" sorry
+lemma interf_12_pre:"\<forall>(R, r) \<in> (atomics p1).(\<forall>P \<in> (assertions p2).\<Turnstile>\<^sub>t\<^sub>r {\<lambda>s. P s \<and> R s} r {P})"
+proof -
+  have "\<turnstile>\<^sub>t\<^sub>r {\<lambda>s. pre20 s \<and> pre10 s} Basic assign11 {pre20}" by simp
+  hence 1:"\<Turnstile>\<^sub>t\<^sub>r {\<lambda>s. pre20 s \<and> pre10 s} Basic assign11 {pre20}" using hoare_sound_tr by blast
+  have "\<turnstile>\<^sub>t\<^sub>r {\<lambda>s. pre21 s \<and> pre10 s} Basic assign11 {pre21}" by simp
+  hence 2:"\<Turnstile>\<^sub>t\<^sub>r {\<lambda>s. pre21 s \<and> pre10 s} Basic assign11 {pre21}" using hoare_sound_tr by blast
+  have "\<turnstile>\<^sub>t\<^sub>r {\<lambda>s. pre22 s \<and> pre10 s} Basic assign11 {pre22}" by simp
+  hence 3:"\<Turnstile>\<^sub>t\<^sub>r {\<lambda>s. pre22 s \<and> pre10 s} Basic assign11 {pre22}" using hoare_sound_tr by blast
+  have "\<turnstile>\<^sub>t\<^sub>r {\<lambda>s. pre23 s \<and> pre10 s} Basic assign11 {pre23}" by simp
+  hence 4:"\<Turnstile>\<^sub>t\<^sub>r {\<lambda>s. pre23 s \<and> pre10 s} Basic assign11 {pre23}" using hoare_sound_tr by blast
+  have "\<turnstile>\<^sub>t\<^sub>r {\<lambda>s. pre24 s \<and> pre10 s} Basic assign11 {pre24}" by simp
+  hence 5:"\<Turnstile>\<^sub>t\<^sub>r {\<lambda>s. pre24 s \<and> pre10 s} Basic assign11 {pre24}" using hoare_sound_tr by blast
+  have "\<turnstile>\<^sub>t\<^sub>r {\<lambda>s. pre20 s \<and> pre11 s} Basic assign12 {pre20}" by simp
+  hence 6:"\<Turnstile>\<^sub>t\<^sub>r {\<lambda>s. pre20 s \<and> pre11 s} Basic assign12 {pre20}" using hoare_sound_tr by blast
+  have "\<turnstile>\<^sub>t\<^sub>r {\<lambda>s. pre21 s \<and> pre11 s} Basic assign12 {pre21}" by simp
+  hence 7:"\<Turnstile>\<^sub>t\<^sub>r {\<lambda>s. pre21 s \<and> pre11 s} Basic assign12 {pre21}" using hoare_sound_tr by blast
+  have "\<turnstile>\<^sub>t\<^sub>r {\<lambda>s. pre22 s \<and> pre11 s} Basic assign12 {pre22}" by simp
+  hence 8:"\<Turnstile>\<^sub>t\<^sub>r {\<lambda>s. pre22 s \<and> pre11 s} Basic assign12 {pre22}" using hoare_sound_tr by blast
+  have "\<turnstile>\<^sub>t\<^sub>r {\<lambda>s. pre23 s \<and> pre11 s} Basic assign12 {pre23}" by simp
+  hence 9:"\<Turnstile>\<^sub>t\<^sub>r {\<lambda>s. pre23 s \<and> pre11 s} Basic assign12 {pre23}" using hoare_sound_tr by blast
+  have "\<turnstile>\<^sub>t\<^sub>r {\<lambda>s. pre24 s \<and> pre11 s} Basic assign12 {pre24}" by simp
+  hence 10:"\<Turnstile>\<^sub>t\<^sub>r {\<lambda>s. pre24 s \<and> pre11 s} Basic assign12 {pre24}" using hoare_sound_tr by blast
+  have "\<turnstile>\<^sub>t\<^sub>r {\<lambda>s. pre20 s \<and> pre13 s} Basic assign13 {pre20}" by simp
+  hence 11:"\<Turnstile>\<^sub>t\<^sub>r {\<lambda>s. pre20 s \<and> pre13 s} Basic assign13 {pre20}" using hoare_sound_tr by blast
+  have "\<turnstile>\<^sub>t\<^sub>r {\<lambda>s. pre21 s \<and> pre13 s} Basic assign13 {pre21}" by simp
+  hence 12:"\<Turnstile>\<^sub>t\<^sub>r {\<lambda>s. pre21 s \<and> pre13 s} Basic assign13 {pre21}" using hoare_sound_tr by blast
+  have "\<turnstile>\<^sub>t\<^sub>r {\<lambda>s. pre22 s \<and> pre13 s} Basic assign13 {pre22}" by simp
+  hence 13:"\<Turnstile>\<^sub>t\<^sub>r {\<lambda>s. pre22 s \<and> pre13 s} Basic assign13 {pre22}" using hoare_sound_tr by blast
+  have "\<turnstile>\<^sub>t\<^sub>r {\<lambda>s. pre23 s \<and> pre13 s} Basic assign13 {pre23}" by simp
+  hence 14:"\<Turnstile>\<^sub>t\<^sub>r {\<lambda>s. pre23 s \<and> pre13 s} Basic assign13 {pre23}" using hoare_sound_tr by blast
+  have "\<turnstile>\<^sub>t\<^sub>r {\<lambda>s. pre24 s \<and> pre13 s} Basic assign13 {pre24}" by simp
+  hence 15:"\<Turnstile>\<^sub>t\<^sub>r {\<lambda>s. pre24 s \<and> pre13 s} Basic assign13 {pre24}" using hoare_sound_tr by blast
+  have "\<turnstile>\<^sub>t\<^sub>r {\<lambda>s. pre20 s \<and> pre14 s} Basic assign14 {pre20}" by simp
+  hence 16:"\<Turnstile>\<^sub>t\<^sub>r {\<lambda>s. pre20 s \<and> pre14 s} Basic assign14 {pre20}" using hoare_sound_tr by blast
+  have "\<turnstile>\<^sub>t\<^sub>r {\<lambda>s. pre21 s \<and> pre14 s} Basic assign14 {pre21}" by simp
+  hence 17:"\<Turnstile>\<^sub>t\<^sub>r {\<lambda>s. pre21 s \<and> pre14 s} Basic assign14 {pre21}" using hoare_sound_tr by blast
+  have "\<turnstile>\<^sub>t\<^sub>r {\<lambda>s. pre22 s \<and> pre14 s} Basic assign14 {pre22}" by simp
+  hence 18:"\<Turnstile>\<^sub>t\<^sub>r {\<lambda>s. pre22 s \<and> pre14 s} Basic assign14 {pre22}" using hoare_sound_tr by blast
+  have "\<turnstile>\<^sub>t\<^sub>r {\<lambda>s. pre23 s \<and> pre14 s} Basic assign14 {pre23}" by simp
+  hence 19:"\<Turnstile>\<^sub>t\<^sub>r {\<lambda>s. pre23 s \<and> pre14 s} Basic assign14 {pre23}" using hoare_sound_tr by blast
+  have "\<turnstile>\<^sub>t\<^sub>r {\<lambda>s. pre24 s \<and> pre14 s} Basic assign14 {pre24}" by simp
+  hence 20:"\<Turnstile>\<^sub>t\<^sub>r {\<lambda>s. pre24 s \<and> pre14 s} Basic assign14 {pre24}" using hoare_sound_tr by blast
+  show ?thesis using 1 2 3 4 5 6 7 8 9 10 11 12 13 14 15 16 17 18 19 20 by auto
+qed
 
 abbreviation Ts::"(acom option \<times> assn) list" where "Ts \<equiv> [(Some p1, post1),(Some p2, post2)]"
 
-lemma "\<turnstile>\<^sub>P {\<lambda>s. \<forall>i \<in> Index Ts. (pre (the (com(Ts!i)))) s} Parallel Ts {\<lambda>s. True}"
+lemma "\<turnstile>\<^sub>P {\<lambda>s. s ''f0'' = 0 \<and> s ''d0'' = 0 \<and> s ''f1'' = 0 \<and> s ''d1'' = 0} Parallel Ts {\<lambda>s. s ''f0'' = 0 \<and> s ''d0'' = 4 \<and> s ''f1'' = 0 \<and> s ''d1'' = 4}"
 proof -
   have Ind:"Index Ts = {0, Suc 0}"
   proof -
@@ -139,6 +241,8 @@ proof -
   qed
   have 0:"(Ts!0) = (Some p1, post1)" by simp
   have 1:"(Ts!1) = (Some p2, post2)" by simp
+  have pre:"(\<lambda> s . \<forall>i \<in> Index Ts. (pre (the (com(Ts!i)))) s) = (\<lambda> s . pre10 s \<and> pre20 s)"  using Ind by force 
+  have post:"(\<lambda> s . \<forall>i \<in> Index Ts. (post (Ts!i)) s) = (\<lambda>s. post1 s \<and> post2 s)"  using Ind by force 
   have "\<turnstile>\<^sub>P {\<lambda> s . \<forall>i \<in> Index Ts. (pre (the (com(Ts!i)))) s} (Parallel Ts) {\<lambda> s . \<forall>i \<in> Index Ts. (post (Ts!i)) s}"
   proof-
     have 2:"(\<forall>i \<in> Index Ts. \<exists>(c::acom) Q. (Ts!i) = (Some c, Q) \<and> (\<turnstile> c {Q}))" using Ind p1_hoare p2_hoare by auto
@@ -164,9 +268,8 @@ proof -
     qed
     thus ?thesis using Ind 0 1 2 by blast
   qed
-  moreover have "\<forall>t. (\<lambda>s. \<forall>i \<in> Index Ts. (post (Ts!i)) s) t \<longrightarrow> (\<lambda>s. True) t" by (smt Ind insertI1 insert_commute nth_Cons_0 nth_Cons_Suc post.simps)
-  moreover have "\<forall>t. (\<lambda> s . \<forall>i \<in> Index Ts. (pre (the (com(Ts!i)))) s) t \<longrightarrow> (\<lambda> s . \<forall>i \<in> Index Ts. (pre (the (com(Ts!i)))) s) t" by blast
-  ultimately show ?thesis using ParConseq by metis
+  hence "\<turnstile>\<^sub>P {\<lambda> s . pre10 s \<and> pre20 s} (Parallel Ts) {\<lambda>s. post1 s \<and> post2 s}" using pre post by auto
+  thus ?thesis using ParConseq by smt
 qed
 
 end
